Small name changes

Sequences/SeqHigherLevel.dfy
@@ -18,13 +18,13 @@ module SeqHigherLevel {
   }
 
   /* Apply an injective function to each element of a sequence. */
-  function method {:opaque} apply_to_set<X(!new), Y>(xs: seq<X>, f: X-->Y): set<Y>
+  function method {:opaque} apply_to_set<X(!new), Y>(s: seq<X>, f: X-->Y): set<Y>
     reads f.reads
     requires forall x :: f.requires(x)
     requires Math.injective(f)
-    ensures forall x :: x in xs <==> f(x) in apply_to_set(xs, f)
+    ensures forall x :: x in s <==> f(x) in apply_to_set(s, f)
   {
-    if |xs| == 0 then {} else apply_to_set(xs[1..], f) + {f(xs[0])}
+    if |s| == 0 then {} else apply_to_set(s[1..], f) + {f(s[0])}
   }
 
   lemma {:opaque} lemma_apply_concat<T,R>(f: (T ~> R), a: seq<T>, b: seq<T>)
